testcases/printtest/exec.c
@@ -28,19 +28,25 @@ int main(){
     pdata->hi = malloc(24);
     void *lo = pdata->lo;
     void *hi = pdata->hi;
-
-    //free(lo);
-    //free(hi);
-
+    free(lo);
+    free(hi);
+    // int init = nondet();
     // test_type i;
     // i.a = 0;
-    // i.b = 100;
+    // i.b = init;
     // int a = i.b;
-
+    // unsigned int c = i.b;
     // int a[10];
     // int num = 101;
     // int b[num+1];
     // a[2] = 111;
     // b[3] = 222;
     // int newname = a[1];
+
+    // DEBUG: free
+    // benchmark
+    // -g compiler option
+    // cfg unroll, variable rename 
+    // memcpy, memset byte level
+    // call graph, variable rename
 } 
